Define monotonic value LR for storeless DOT!

ecoop17/dot_storeless_wfrel.v
@@ -1,57 +1,68 @@
-Require Import dot_storeless_tidy.
 Require Import Omega.
-Require Import tactics.
+Require Import Coq.Relations.Relation_Operators.
+Require Import Coq.Wellfounded.Lexicographic_Product.
+Require Import Equations.Equations.
 
+Require Import dot_storeless_tidy.
+Require Import tactics.
 (* Require Import dot_monads. *)
+
+(*******************)
+(* Define language infrastructure. *)
+
+(*******************)
+(* Renames for adaption. *)
 
 Definition tsize_flat := tsize.
 
-Definition val_type_measure T (k : nat) := (existT (fun _ => nat) k (tsize_flat T)).
-Hint Unfold val_type_measure.
-
+Lemma open_preserves_size': forall T v j,
+    tsize_flat (open j v T) = tsize_flat T.
+Proof. unfold tsize_flat; intros; rewrite <- open_preserves_size; easy. Qed.
 Definition vl := tm.
-Definition vset := vl -> Prop.
-Hint Unfold vset.
 
-Require Import Coq.Relations.Relation_Operators.
-Require Import Coq.Wellfounded.Lexicographic_Product.
+Definition closed_ty i j T := closed j i T.
+Definition wf {A} (G : list A) T := closed_ty 0 (length G) T.
+
+(*******************)
+(* Small-step semantics *)
+Inductive steps t0 : tm -> nat -> Prop :=
+| Step0 : steps t0 t0 0
+| StepS : forall t1 t2 i, step t0 t1 -> steps t1 t2 i -> steps t0 t2 (S i).
+
+Definition irred t0 := not (exists t1, step t0 t1).
+
+(* Definition env_prop := list vl ->  Prop. *)
+(* Hint Unfold env_prop. *)
+
+Definition vl_prop := vl -> Prop.
+Hint Unfold vl_prop.
+
+Definition pretype_dom n :=
+  forall (n0: nat) (H: n0 <= n), vl_prop.
+Hint Unfold pretype_dom.
+
 Hint Constructors lexprod.
 
-Set Implicit Arguments.
-Check lexprod.
-Definition termRel := lexprod nat (fun _ => nat) lt (fun _ => lt).
-Hint Unfold termRel.
-
-Lemma wf_termRel : well_founded termRel.
-Proof.
- apply wf_lexprod; intro; apply lt_wf.
-Defined.
-Hint Resolve wf_termRel.
-
+(*******************)
 (* Infrastructure for well-founded induction for properties of vtp. *)
-Definition argPair := (ty * nat)%type.
+Definition argMeasure (p: ty * nat) := let '(T, n) := p in (existT (fun _ => nat) n (tsize_flat T)).
+Definition val_type_termRel := MR (lexprod lt (fun _ => lt)) (fun p => let '(T, n) := p in (existT (fun _ => nat) n (tsize_flat T))).
 
-Definition argMeasure (p: argPair) := let '(T, n) := p in val_type_measure T n.
-Definition val_type_termRel := MR termRel argMeasure.
-
-Lemma wf_val_type_termRel : well_founded val_type_termRel.
-Proof.
-  apply measure_wf. apply wf_termRel.
-Qed.
-Hint Resolve wf_val_type_termRel.
-
+(*******************)
+(* Tactics. *)
 (* Show that different branches are disjoint. *)
 Ltac discriminatePlus :=
-  (* repeat split; intros; let Habs := fresh "Habs" in intro Habs; destruct Habs; discriminate. *)
-  repeat split_conj; intros;
-  (let Habs := fresh "Habs" in
-  try (intro Habs; destruct Habs) + idtac);
-  discriminate.
+  idtac.
+  (* (* repeat split; intros; let Habs := fresh "Habs" in intro Habs; destruct Habs; discriminate. *) *)
+  (* repeat split_conj; intros; *)
+  (* (let Habs := fresh "Habs" in *)
+  (* try (intro Habs; destruct Habs) + idtac); *)
+  (* discriminate. *)
 
 (* Prove some inequalities needed below, without producing big proof terms like omega does. Probably not worth it. *)
 Ltac simple_ineq :=
   (* simpl; omega. *)
-  simpl; auto using le_n_S, le_plus_l, le_plus_r; omega.
+  simpl; auto using le_n_S, le_plus_l, le_plus_r; abstract omega.
   (* If this tactic fails, add back omega at the end. *)
 
 (* These three lemmas take care of the various forms of proof obligations that arise from val_type. *)
@@ -59,39 +70,29 @@ Lemma termRelShow: forall j n T1 T2,
   j <= n -> tsize_flat T2 < tsize_flat T1 ->
   val_type_termRel (T2, j) (T1, n).
 Proof.
-  intros * Hj Ht.
-  unfold val_type_termRel, MR, termRel, argMeasure, val_type_measure.
+  intros * Hj Ht; unfold val_type_termRel, MR, argMeasure;
   (* If we only know that Hj: j <= n, we must case-split on it, and use
      smaller_types when j = n and smaller_n when j < n. *)
-  destruct Hj; try assert (j < S m) by simple_ineq; auto.
+    destruct Hj; try assert (j < S m) by simple_ineq; auto.
 Qed.
-  (* - apply right_lex. assumption. *)
-  (* - apply left_lex. omega. *)
 
 Hint Extern 5 (_ < tsize_flat _) =>
-  unfold open;
-  rewrite <- open_preserves_size;
+  rewrite open_preserves_size';
   simple_ineq.
-
 
 Lemma termRelShowOpen: forall j n x T1 T2,
   j <= n -> tsize_flat T2 < tsize_flat T1 ->
-  val_type_termRel (open 0 (VarF x) T2, j) (T1, n).
+  val_type_termRel (open 0 x T2, j) (T1, n).
 Proof.
-  intros * Hj Ht.
-  unfold val_type_termRel, MR, termRel, argMeasure, val_type_measure.
-  destruct Hj; try assert (j < S m) by simple_ineq; auto.
-  (* unfold open; try rewrite open_preserves_size'. *)
-  (* auto using left_lex, right_lex. *)
+  intros * Hj Ht; unfold val_type_termRel, MR, argMeasure;
+    destruct Hj; try assert (j < S m) by simple_ineq; auto.
 Qed.
 
 Lemma termRelShowLt: forall j n T1 T2,
   j < n ->
   val_type_termRel (T2, j) (T1, n).
 Proof.
-  intros * Hj.
-  unfold val_type_termRel, MR, termRel, argMeasure, val_type_measure.
-  auto.
+  intros * Hj; unfold val_type_termRel, MR, argMeasure; auto.
 Qed.
 
 Ltac applyNSimpleIneq l := apply l; simple_ineq.
@@ -118,43 +119,13 @@ Ltac valTypeObligations Hj :=
   Tactics.program_simpl;
   solve [ smaller_n | smaller_types | discriminatePlus | (try destruct Hj; [ smaller_types | smaller_n ])].
 
-(* Definition env_prop := list vl ->  Prop. *)
-(* Hint Unfold env_prop. *)
-
-Definition vl_prop := vl -> Prop.
-Hint Unfold vl_prop.
-
-Definition smaller_args T0 n0 T n :=
-  termRel (val_type_measure T0 n0) (val_type_measure T n).
-Hint Unfold smaller_args.
-
-Definition pretype_dom n :=
-  forall (n0: nat) (H: n0 <= n), vl_prop.
-Hint Unfold pretype_dom.
-
-Definition closed_ty i j T := closed j i T.
-Definition wf {A} (G : list A) T := closed_ty 0 (length G) T.
-
-Check dot_storeless_tidy.step.
-Inductive steps t0 : tm -> nat -> Prop :=
-| Step0 : steps t0 t0 0
-| StepS : forall t1 t2 i, step t0 t1 -> steps t1 t2 i -> steps t0 t2 (S i).
-
-Definition irred t0 := not (exists t1, step t0 t1).
-
-
 Local Obligation Tactic := valTypeObligationsSSReflection.
-From Equations Require Import Equations.
-Equations expr_sem {n} (T : ty) (A : pretype_dom n) k (p : k <= n) (t : tm) : Prop :=
-  expr_sem T A k p t :=
-  (* If evaluation terminates in at most k steps without running out of fuel, *)
-  closed_ty 0 0 T /\
-  forall v j,
-    steps t v j ->
-    irred v ->
-    j <= k ->
-    (* then evaluation did not get stuck and the result satisfies A. *)
-    exists v, A (k - j) _ v.
+Require Import Equations.Equations.
+
+Lemma wf_val_type_termRel : well_founded val_type_termRel.
+Proof. apply measure_wf; apply wf_lexprod; intro; apply lt_wf. Qed.
+Hint Resolve wf_val_type_termRel.
+Instance WF_val_type_termRel: WellFounded val_type_termRel := wf_val_type_termRel.
 
 (* Program Definition expr_sem {n} T (A : pretype_dom n) k (p : k <= n) t : Prop := *)
 (*   (* If evaluation terminates in at most k steps without running out of fuel, *) *)
@@ -166,15 +137,302 @@ Equations expr_sem {n} (T : ty) (A : pretype_dom n) k (p : k <= n) (t : tm) : Pr
 (*     (* then evaluation did not get stuck and the result satisfies A. *) *)
 (*     exists v, A (k - j) _ v. *)
 
-Instance WF_val_type_termRel: WellFounded val_type_termRel := wf_val_type_termRel.
+(* Equations val_type (Tn: ty * nat) (t : tm) : Prop := *)
+(*   val_type Tn t by rec Tn val_type_termRel := *)
+(*     val_type (pair T O) t := True; *)
+(*     val_type (pair T (S n)) t := val_type (pair T n) t. *)
 
-Equations val_type (Tn: argPair) (t : tm) : Prop :=
+(* Next Obligation. Qed. *)
+(* Next Obligation. induction n; simp val_type. Defined. *)
+
+(* Infrastructure for well-founded induction for properties of vtp. *)
+Lemma ind_args : forall (P: ty -> nat -> Prop),
+    (forall T n,
+        (forall T' n', val_type_termRel (T', n') (T, n) -> P T' n') -> P T n) ->
+    forall T n, P T n.
+Proof.
+  intros * Hind *.
+  pose (p := (T, n));
+  replace T with (fst p) by reflexivity;
+  replace n with (snd p) by reflexivity;
+  generalize dependent p;
+  clear T n.
+  eapply well_founded_ind; eauto.
+  intros p1 Hless.
+  destruct p1 as [T n]; simpl in *.
+  apply Hind.
+  intros *.
+  apply Hless.
+Qed.
+
+Ltac vtp_induction T n :=
+  apply ind_args with (T := T) (n := n);
+  clear T n.
+
+Equations expr_sem n (T : ty) (A : pretype_dom n) k (p : k <= n) (t : tm) : Prop :=
+  expr_sem n T A k p t :=
+  (* If evaluation terminates in at most k steps without running out of fuel, *)
+  closed_ty 0 0 T /\
+  forall v j,
+    steps t v j ->
+    irred v ->
+    j <= k ->
+    (* then evaluation did not get stuck and the result satisfies A. *)
+    exists v, A (k - j) _ v.
+
+
+Equations val_type (Tn: ty * nat) (v : tm) : Prop :=
   val_type Tn t by rec Tn val_type_termRel :=
-    val_type (pair T (S n)) t := val_type (pair T n) t;
-    val_type (pair T O) t := True.
+    val_type (pair TBot n) v := False;
+    val_type (pair TTop n) v := True;
+    val_type (pair (TFun l T1 T2) n) (tvar (VObj ds)) :=
+                                  closed_ty 0 0 T1 /\ closed_ty 1 0 T2 /\
+                                  exists U1 U2 t,
+                                    index l (dms_to_list (subst_dms ds ds)) = Some (dfun U1 U2 t) /\
+                                    (forall vyds k (Hj: k < n),
+                                        val_type (pair T1 k) (tvar (VObj vyds)) ->
+                                        expr_sem k
+                                          (open 0 (VObj vyds) T2)
+                                          (fun kj p t => val_type (open 0 (VObj vyds) T2, kj) t)
+                                          k _ t);
+    val_type (pair (TMem l L U) n) (tvar (VObj ds)) :=
+                                       closed_ty 0 0 L /\ closed_ty 0 0 U /\
+                                       exists TX, index l (dms_to_list (subst_dms ds ds)) = Some (dty TX) /\
+                                             (forall vy j (Hj: j <= n), val_type (pair L j) vy -> val_type (pair U j) vy) /\
+                                             (forall vy j (Hj: j < n),
+                                                 (val_type (pair L j) vy -> val_type (pair TX j) vy) /\
+                                                 (val_type (pair TX j) vy -> val_type (pair U j) vy));
+    val_type (pair (TSel (VObj ds) l) n) v :=
+                                         dms_closed 0 1 ds /\
+                                         exists TX, index l (dms_to_list (subst_dms ds ds)) = Some (dty TX) /\
+                                               forall j (Hj: j < n), val_type (TX, j) v;
+    val_type (pair (TBind T) n) (tvar (VObj ds)) :=
+                                           closed_ty 1 0 T /\
+                                           val_type (pair (open 0 (VObj ds) T) n) (tvar (VObj ds));
+    val_type (pair (TAnd T1 T2) n) v := val_type (pair T1 n) v /\ val_type (pair T2 n) v;
+    val_type (pair (TOr T1 T2) n) v :=
+                                             closed_ty 0 0 T1 /\ closed_ty 0 0 T2 /\
+                                             (val_type (pair T1 n) v \/ val_type (pair T2 n) v);
+    val_type (pair T n) v := False.
 
-Next Obligation. Qed.
+Solve Obligations with valTypeObligationsSSReflection. (* Works *)
+(* Solve All Obligations. (* No effect *) *)
+(* Next Obligation. Qed. (* Works for 1 obligation. *) *)
+
 Next Obligation.
-  destruct Tn as [? n]; induction n;
-    simp val_type.
+  Transparent val_type_unfold.
+  Ltac loop := (subst; progress (better_case_match; simp val_type); loop) || idtac.
+  apply ind_args with (T := t) (n := n); clear t n; intros * Hind;
+    rewrite val_type_unfold_eq; unfold val_type_unfold; loop;
+      constructors; apply Hind; valTypeObligationsSSReflection.
+    (* rewrite val_type_unfold_eq in *. unfold val_type_unfold in *. simpl. auto. *)
+  (* - constructors; rewrite val_type_unfold_eq in *; unfold val_type_unfold in *; easy. *)
+  Opaque val_type_unfold.
 Defined.
+
+Definition vtp T n v := val_type (T, n) v.
+Hint Unfold vtp.
+Example ex0 : forall n v, vtp TTop n v.
+Proof.
+  intros; autounfold; now simp val_type.
+Qed.
+
+Hint Constructors closed.
+Hint Unfold closed_ty.
+Example ex3: forall T n, vtp (TMem 0 TBot TTop) n (tvar (VObj (dcons (dty T) dnil))).
+Proof.
+  intros; autounfold; simp val_type; intuition eauto; simpl;
+  eexists; intuition eauto; now simp val_type in *.
+Qed.
+
+(* (* Check syntax_mutind. *) *)
+(* Check closed_mutind. *)
+(* Lemma open_closed : *)
+(*   (forall i jv T i j k, closed i j (open k v T) -> closed i (S j) T). *)
+(*   (* (forall v T i j k, vr_closed i j (open k v T) -> closed i (S j) T) /\ *) *)
+(* Proof. *)
+(*   induction T; simpl in *; constructor; try easy; *)
+(*     inversion H; subst; eauto. *)
+(*   (* inversion H; subst; eauto. *) *)
+(*   (* repeat better_case_match; try constructor; inverts H. *) *)
+(* Admitted. *)
+(* (* Lemma open_closed : *) *)
+(* (*   (forall v T i j k, closed i j (open k v T) -> closed i (S j) T). *) *)
+(* (*   (* (forall v T i j k, vr_closed i j (open k v T) -> closed i (S j) T) /\ *) *) *)
+(* (* Proof. *) *)
+(* (*   induction T; simpl in *; constructor; try easy; *) *)
+(* (*     inversion H; subst; eauto. *) *)
+(* (*   (* inversion H; subst; eauto. *) *) *)
+(* (*   (* repeat better_case_match; try constructor; inverts H. *) *) *)
+(* (* Admitted. *) *)
+
+Hint Constructors vr_closed.
+Hint Constructors dms_closed.
+(* Hint Extern 100 (val_type_termRel _ _) => *)
+(*   valTypeObligationsSSReflection. *)
+Lemma vtp_closed: forall T n v,
+    vtp T n v -> closed_ty 0 0 T.
+Proof.
+  unfold vtp, closed_ty;
+  intros *; vtp_induction T n; intros;
+    destruct T;
+    destruct v;
+    simp val_type in *; ev;
+      try eauto || easy.
+  all: (destruct v0 || destruct v; simp val_type in *; ev; now eauto) ||
+           constructor; eapply H; smaller_types.
+Qed.
+  (* (* all: try solve [destruct v; simp val_type in *; ev; now eauto]. *) *)
+  (* (* all: try solve *) *)
+  (* (*       [ destruct v; simp val_type in *; ev; now eauto | *) *)
+  (* (*         destruct v0; simp val_type in *; ev; now eauto | *) *)
+  (* (*         constructor; eapply H; smaller_types *) *)
+  (* (*       ]. *) *)
+  (* (* intuition eauto. *) *)
+  (* (* intuition eauto. *) *)
+  (* - destruct v; simp val_type in *; ev; now eauto. *)
+  (* - destruct v; simp val_type in *; ev; now eauto. *)
+  (* - destruct v0; simp val_type in *; ev; now eauto. *)
+  (* - destruct v0; simp val_type in *; ev; now eauto. *)
+  (* - destruct v; simp val_type in *; ev; now eauto. *)
+  (*   (* assert (closed 0 0 (open 0 (VObj d) T)). { *) *)
+  (*   (*   eapply H; valTypeObligationsSSReflection. *) *)
+  (*   (* } *) *)
+  (*   (* eauto using open_closed. *) *)
+  (* - *)
+  (*   constructor. *)
+  (*   eapply H. smaller_types. *)
+  (*   intuition (try smaller_types || eauto). *)
+  (* - constructor; eapply H; smaller_types. *)
+  (* (* - destruct H0. constructor; eapply H; valTypeObligationsSSReflection. *) *)
+  (* (* - constructor; eapply H; valTypeObligationsSSReflection. *) *)
+  (* (* - destruct v. try easy; *) *)
+  (* (*     try destruct v; simp val_type in *; ev; now eauto. *) *)
+  (* (*   (* Either case_match or better_case_match works*) *) *)
+  (* (*   repeat better_case_match; ev; eauto 6. *) *)
+  (* (*     contradiction. *) *)
+  (* (* unfold vtp; intros *; *) *)
+  (* (* apply ind_args with (T := T) (n := n); clear T n; intros * Hind ?. *) *)
+  (* (* funind val_type Hind. *) *)
+  (* (* induction T; intros; destruct v; vtp_simpl_unfold; ev; try eauto; *) *)
+  (* (*   (* Either case_match or better_case_match works*) *) *)
+  (* (*   repeat better_case_match; ev; eauto 6; *) *)
+  (* (*     contradiction. *) *)
+
+Lemma vtp_mon: forall T v m n,
+    vtp T n v ->
+    m <= n ->
+    vtp T m v.
+Proof.
+  unfold vtp.
+  intros *. revert m.
+  funind (val_type (T, n) v) Hcall.
+  all: intros; simp val_type; ev;
+    unfold closed_ty in *;
+    simp expr_sem in *;
+    repeat split_conj; eauto; try easy.
+
+  - do 3 eexists; split_conj; eauto; intros;
+    lets Hfunsucceeds: H3 ___; eauto.
+    Unshelve.
+    omega.
+
+  - eexists; split_conj; eauto.
+
+  - match goal with
+    | [ H : val_type _ _ \/ val_type _ _ |- _ ] => destruct H
+    end; eauto.
+Qed.
+
+Hint Resolve vtp_mon.
+  (* - case_or_vtp; eauto. *)
+  (*   Hint Constructors or. *)
+  (*   intuition (mon_induct_step Hind n). *)
+  (* Ltac mon_induct_step Hind n := (try (apply Hind with (n' := n); try smaller_types; assumption)). *)
+  (* - *)
+  (*   intros. *)
+
+  (*   lets Hfunsucceeds: H3 ___. eauto. eauto. *)
+  (*     assert (Hk: k < n0) by omega; specialize (H3 vyds k Hk H4); simp expr_sem in H3; *)
+  (*       ev; eauto. *)
+  (*   lets (vr & Hworks): H8 ___; eauto; ev. eapply Hworks. *)
+  (*   eapply H8. *)
+
+  (*   firstorder eauto. *)
+
+  (* lets H: (H3 vyds k). *)
+  (* do 3 eexists; repeat split_conj; eauto. *)
+  (* eexists. *)
+  (* repeat eexists; eauto. *)
+  (* - clear Hcall. *)
+  (*   unfold closed_ty in *. eapply closed_open; simpl. assumption. *)
+  (* eauto using closed_open, closed_upgrade. *)
+  (* Check closed_open. *)
+  (* Check closed_upgrade. *)
+
+  (* (* Check val_type_ind_fun. *) *)
+  (* (* induction (val_type_ind_fun (T, n) v). *) *)
+
+  (* (* Print FunctionalInduction_val_type. *) *)
+  (* (* funind val_type Hcall. *) *)
+  (* (*   intros *; revert v m; *) *)
+  (* (*   vtp_induction T n; intros * Hind * Hvtpn1 * Hmn. *) *)
+  (* (* destruct T; destruct v; simp val_type in *; ev; repeat split_conj. *) *)
+
+Definition venv := list dms.
+Definition tenv := list ty.
+Hint Unfold venv.
+Hint Unfold tenv.
+
+Inductive R_env (k : nat) : venv -> tenv -> Set :=
+  (* (env: venv) (G: tenv) : Set := *)
+| R_nil :
+    R_env k [] []
+| R_cons : forall T v env G,
+    R_env k env G ->
+    vtp (open 0 (VObj v) T) k (tvar (VObj v)) ->
+    R_env k (v :: env) (T :: G)
+.
+Hint Constructors R_env.
+
+Lemma R_env_mon: forall G env m n,
+    R_env n env G ->
+    m <= n ->
+    R_env m env G.
+Proof.
+  intros * Henv; induction Henv; eauto.
+Qed.
+Hint Resolve R_env_mon.
+
+Lemma wf_length : forall k vs ts,
+                    R_env k vs ts ->
+                    (length vs = length ts).
+Proof.
+  intros * H; induction H; simpl; congruence.
+Qed.
+
+Program Definition etp0 T k e :=
+  expr_sem k T (fun k _ => vtp T k) k _ e.
+
+Lemma etp0_closed: forall T k v,
+    etp0 T k v -> closed_ty 0 0 T.
+Proof.
+  unfold etp0; intros; simp expr_sem in *; tauto.
+Qed.
+Hint Resolve etp0_closed.
+
+(* Fixpoint subst_all_ty (env : venv) (T: ty) := *)
+(*   match env with *)
+(*   | [] => T *)
+(*   | v :: vs => *)
+(*     subst_all_ty vs (open (length vs) (VObj v) T) *)
+(*   end. *)
+
+(* Goal forall l dms, subst_all_ty [dms] (TSel (VarB 0) l) = TSel (VObj dms) l. *)
+(*   easy. *)
+(* Qed. *)
+(* Goal forall l dms0 dms1, subst_all_ty [dms1, dms0] (TSel (VarB 1) l) = TSel (VObj dms1) l. *)
+(*   simpl. *)
+(*   easy. *)
+(* Qed. *)
+
